@prefix : <https://github.com/leonardozilli/Bias_Ontology/BizarrenessEffect#> .
@prefix fs: <https://w3id.org/framester/data/framestercore/> .
@prefix cbo: <https://github.com/leonardozilli/Bias_Ontology/BizarrenessEffect#> .
@prefix owl: <http://www.w3.org/2002/07/owl#> .
@prefix rdf: <http://www.w3.org/1999/02/22-rdf-syntax-ns#> .
@prefix xml: <http://www.w3.org/XML/1998/namespace> .
@prefix xsd: <http://www.w3.org/2001/XMLSchema#> .
@prefix rdfs: <http://www.w3.org/2000/01/rdf-schema#> .
@base <https://github.com/leonardozilli/Bias_Ontology/BizarrenessEffect> .

<https://github.com/leonardozilli/Bias_Ontology/BizarrenessEffect> rdf:type owl:Ontology ;
                                                                    owl:imports <https://raw.githubusercontent.com/modellingDH/odp_experience/master/owl/cp_experience.owl.ttl> ;
                                                                    <http://purl.org/dc/terms/created> "2023-07-23" ;
                                                                    <http://purl.org/dc/terms/creator> "Leonardo Zilli" ;
                                                                    <http://purl.org/dc/terms/description> "The Bizarreness effect module of the Cognitive Bias Ontology." ;
                                                                    <http://purl.org/dc/terms/title> "Bizarreness effect ontology" ;
                                                                    rdfs:comment "The Bizarreness effect is the tendency of bizarre material to be better remembered than common material." .

#################################################################
#    Annotation properties
#################################################################

###  http://purl.org/dc/terms/created
<http://purl.org/dc/terms/created> rdf:type owl:AnnotationProperty .


#################################################################
#    Classes
#################################################################

###  https://github.com/leonardozilli/Bias_Ontology/BizarrenessEffect#BizarreContent
cbo:BizarreContent rdf:type owl:Class ;
                   owl:equivalentClass fs:Prominence ;
                   rdfs:subClassOf cbo:MentalContent .


###  https://github.com/leonardozilli/Bias_Ontology/BizarrenessEffect#MentalContent
cbo:MentalContent rdf:type owl:Class ;
                  rdfs:subClassOf <http://modellingdh.github.io/ont/odp/term/Prompt> .


###  https://w3id.org/framester/data/framestercore/ExperiencerObj
fs:ExperiencerObj rdf:type owl:Class ;
                  rdfs:subClassOf <http://modellingdh.github.io/ont/odp/term/Engagement> ;
                  rdfs:comment "Some phenomenon (the Stimulus) provokes a particular emotion in an Experiencer. Nightmare on Elm Street scared me silly." .


###  https://w3id.org/framester/data/framestercore/Memory
fs:Memory rdf:type owl:Class ;
          rdfs:subClassOf <http://ontology.eil.utoronto.ca/icity/ActivitySpecification/Activity> ;
          rdfs:comment "This frame is concerned with Cognizers remembering and forgetting mental Content." .


###  https://w3id.org/framester/data/framestercore/Prominence
fs:Prominence rdf:type owl:Class ;
              rdfs:subClassOf fs:Memory ;
              rdfs:comment "An Entity stands out perceptually in comparison to other members of its type." .


###  https://w3id.org/framester/data/framestercore/Typicality
fs:Typicality rdf:type owl:Class ;
              rdfs:subClassOf <http://modellingdh.github.io/ont/odp/term/Observation> ;
              rdfs:comment "An Entity is generally, or with regard to a particular Feature, representative of the Comparison_set of which it is a member." .


#################################################################
#    Individuals
#################################################################

###  https://github.com/leonardozilli/Bias_Ontology/BizarrenessEffect#bizarre_article
cbo:bizarre_article rdf:type owl:NamedIndividual ,
                             cbo:BizarreContent .


###  https://github.com/leonardozilli/Bias_Ontology/BizarrenessEffect#decoded_prominent_memory
cbo:decoded_prominent_memory rdf:type owl:NamedIndividual ,
                                      fs:Prominence .


###  https://github.com/leonardozilli/Bias_Ontology/BizarrenessEffect#emotional_stimulus
cbo:emotional_stimulus rdf:type owl:NamedIndividual ,
                                fs:ExperiencerObj ;
                       <http://modellingdh.github.io/ont/odp/term/inActivity> cbo:memory_encoding .


###  https://github.com/leonardozilli/Bias_Ontology/BizarrenessEffect#memory_encoding
cbo:memory_encoding rdf:type owl:NamedIndividual ,
                             fs:Memory .


###  https://github.com/leonardozilli/Bias_Ontology/BizarrenessEffect#mundane_article
cbo:mundane_article rdf:type owl:NamedIndividual ,
                             cbo:MentalContent .


###  https://github.com/leonardozilli/Bias_Ontology/BizarrenessEffect#newspaper_reader
cbo:newspaper_reader rdf:type owl:NamedIndividual ,
                              <http://www.ontologydesignpatterns.org/cp/owl/persons.owl#Person> ;
                     <http://modellingdh.github.io/ont/odp/term/isEngagedIn> cbo:emotional_stimulus .


###  Generated by the OWL API (version 4.5.25.2023-02-15T19:15:49Z) https://github.com/owlcs/owlapi
