<?xml version="1.0"?>
<rdf:RDF xmlns="https://github.com/leonardozilli/CognitiveBiasOntology/HumorEffect#"
     xml:base="https://github.com/leonardozilli/CognitiveBiasOntology/HumorEffect"
     xmlns:fs="https://w3id.org/framester/data/framestercore/"
     xmlns:cbo="https://github.com/leonardozilli/CognitiveBiasOntology/HumorEffect#"
     xmlns:owl="http://www.w3.org/2002/07/owl#"
     xmlns:rdf="http://www.w3.org/1999/02/22-rdf-syntax-ns#"
     xmlns:xml="http://www.w3.org/XML/1998/namespace"
     xmlns:xsd="http://www.w3.org/2001/XMLSchema#"
     xmlns:rdfs="http://www.w3.org/2000/01/rdf-schema#"
     xmlns:term="http://modellingdh.github.io/ont/odp/term/"
     xmlns:terms="http://purl.org/dc/terms/"
     xmlns:cpannotationschema="http://www.ontologydesignpatterns.org/schemas/cpannotationschema.owl#">
    <owl:Ontology rdf:about="https://github.com/leonardozilli/CognitiveBiasOntology/HumorEffect">
        <owl:imports rdf:resource="https://raw.githubusercontent.com/modellingDH/odp_experience/master/owl/cp_experience.owl.ttl"/>
        <terms:created>2023-07-23</terms:created>
        <terms:creator>Leonardo Zilli</terms:creator>
        <terms:description>The Humor effect module of the Cognitive Bias Ontology.</terms:description>
        <terms:title>Humor effect ontology</terms:title>
        <rdfs:comment>Scenario:
A company creates a humorous television commercial for their product. The funny storyline and witty dialogue engage viewers, making the advertisement more memorable. As a result, consumers are more likely to remember the product and its key features when making purchasing decisions.</rdfs:comment>
        <rdfs:comment>The humor effect is the tendencye of humorous material to be better remembered than common material.</rdfs:comment>
    </owl:Ontology>
    


    <!-- 
    ///////////////////////////////////////////////////////////////////////////////////////
    //
    // Annotation properties
    //
    ///////////////////////////////////////////////////////////////////////////////////////
     -->

    


    <!-- http://purl.org/dc/terms/created -->

    <owl:AnnotationProperty rdf:about="http://purl.org/dc/terms/created"/>
    


    <!-- 
    ///////////////////////////////////////////////////////////////////////////////////////
    //
    // Classes
    //
    ///////////////////////////////////////////////////////////////////////////////////////
     -->

    


    <!-- https://github.com/leonardozilli/CognitiveBiasOntology/HumorEffect#Humor -->

    <owl:Class rdf:about="https://github.com/leonardozilli/CognitiveBiasOntology/HumorEffect#Humor">
        <rdfs:subClassOf rdf:resource="https://w3id.org/framester/data/framestercore/Feeling"/>
    </owl:Class>
    


    <!-- https://github.com/leonardozilli/CognitiveBiasOntology/HumorEffect#HumorousContent -->

    <owl:Class rdf:about="https://github.com/leonardozilli/CognitiveBiasOntology/HumorEffect#HumorousContent">
        <owl:equivalentClass rdf:resource="https://w3id.org/framester/data/framestercore/Prominence"/>
        <rdfs:subClassOf rdf:resource="https://github.com/leonardozilli/CognitiveBiasOntology/HumorEffect#MentalContent"/>
    </owl:Class>
    


    <!-- https://github.com/leonardozilli/CognitiveBiasOntology/HumorEffect#MentalContent -->

    <owl:Class rdf:about="https://github.com/leonardozilli/CognitiveBiasOntology/HumorEffect#MentalContent">
        <rdfs:subClassOf rdf:resource="http://modellingdh.github.io/ont/odp/term/Prompt"/>
    </owl:Class>
    


    <!-- https://w3id.org/framester/data/framestercore/ExperiencerObj -->

    <owl:Class rdf:about="https://w3id.org/framester/data/framestercore/ExperiencerObj">
        <rdfs:subClassOf rdf:resource="http://modellingdh.github.io/ont/odp/term/Engagement"/>
        <rdfs:comment>Some phenomenon (the Stimulus) provokes a particular emotion in an Experiencer. Nightmare on Elm Street scared me silly.</rdfs:comment>
    </owl:Class>
    


    <!-- https://w3id.org/framester/data/framestercore/Feeling -->

    <owl:Class rdf:about="https://w3id.org/framester/data/framestercore/Feeling">
        <rdfs:subClassOf rdf:resource="http://modellingdh.github.io/ont/odp/term/Observation"/>
        <rdfs:comment>In this frame an Experiencer experiences an Emotion or is in an Emotional_state.</rdfs:comment>
    </owl:Class>
    


    <!-- https://w3id.org/framester/data/framestercore/Memory -->

    <owl:Class rdf:about="https://w3id.org/framester/data/framestercore/Memory">
        <rdfs:subClassOf rdf:resource="http://ontology.eil.utoronto.ca/icity/ActivitySpecification/Activity"/>
        <rdfs:comment>This frame is concerned with Cognizers remembering and forgetting mental Content.</rdfs:comment>
    </owl:Class>
    


    <!-- https://w3id.org/framester/data/framestercore/Prominence -->

    <owl:Class rdf:about="https://w3id.org/framester/data/framestercore/Prominence">
        <rdfs:subClassOf rdf:resource="https://w3id.org/framester/data/framestercore/Memory"/>
        <rdfs:comment>An Entity stands out perceptually in comparison to other members of its type.</rdfs:comment>
    </owl:Class>
    


    <!-- 
    ///////////////////////////////////////////////////////////////////////////////////////
    //
    // Individuals
    //
    ///////////////////////////////////////////////////////////////////////////////////////
     -->

    


    <!-- https://github.com/leonardozilli/CognitiveBiasOntology/HumorEffect#consumer -->

    <owl:NamedIndividual rdf:about="https://github.com/leonardozilli/CognitiveBiasOntology/HumorEffect#consumer">
        <rdf:type rdf:resource="http://www.ontologydesignpatterns.org/cp/owl/persons.owl#Person"/>
        <term:isEngagedIn rdf:resource="https://github.com/leonardozilli/CognitiveBiasOntology/HumorEffect#emotional_stimulus"/>
    </owl:NamedIndividual>
    


    <!-- https://github.com/leonardozilli/CognitiveBiasOntology/HumorEffect#decoded_prominent_memory -->

    <owl:NamedIndividual rdf:about="https://github.com/leonardozilli/CognitiveBiasOntology/HumorEffect#decoded_prominent_memory">
        <rdf:type rdf:resource="https://w3id.org/framester/data/framestercore/Prominence"/>
    </owl:NamedIndividual>
    


    <!-- https://github.com/leonardozilli/CognitiveBiasOntology/HumorEffect#emotional_stimulus -->

    <owl:NamedIndividual rdf:about="https://github.com/leonardozilli/CognitiveBiasOntology/HumorEffect#emotional_stimulus">
        <rdf:type rdf:resource="https://w3id.org/framester/data/framestercore/ExperiencerObj"/>
        <term:inActivity rdf:resource="https://github.com/leonardozilli/CognitiveBiasOntology/HumorEffect#memory_encoding"/>
    </owl:NamedIndividual>
    


    <!-- https://github.com/leonardozilli/CognitiveBiasOntology/HumorEffect#humorous_advertisement -->

    <owl:NamedIndividual rdf:about="https://github.com/leonardozilli/CognitiveBiasOntology/HumorEffect#humorous_advertisement">
        <rdf:type rdf:resource="https://github.com/leonardozilli/CognitiveBiasOntology/HumorEffect#HumorousContent"/>
        <term:producedObservation rdf:resource="https://github.com/leonardozilli/CognitiveBiasOntology/HumorEffect#laugh"/>
    </owl:NamedIndividual>
    


    <!-- https://github.com/leonardozilli/CognitiveBiasOntology/HumorEffect#laugh -->

    <owl:NamedIndividual rdf:about="https://github.com/leonardozilli/CognitiveBiasOntology/HumorEffect#laugh">
        <rdf:type rdf:resource="https://github.com/leonardozilli/CognitiveBiasOntology/HumorEffect#Humor"/>
        <term:isReflectionOn rdf:resource="https://github.com/leonardozilli/CognitiveBiasOntology/HumorEffect#emotional_stimulus"/>
    </owl:NamedIndividual>
    


    <!-- https://github.com/leonardozilli/CognitiveBiasOntology/HumorEffect#memory_encoding -->

    <owl:NamedIndividual rdf:about="https://github.com/leonardozilli/CognitiveBiasOntology/HumorEffect#memory_encoding">
        <rdf:type rdf:resource="https://w3id.org/framester/data/framestercore/Memory"/>
    </owl:NamedIndividual>
    


    <!-- https://github.com/leonardozilli/CognitiveBiasOntology/HumorEffect#mundane_advertisement -->

    <owl:NamedIndividual rdf:about="https://github.com/leonardozilli/CognitiveBiasOntology/HumorEffect#mundane_advertisement">
        <rdf:type rdf:resource="https://github.com/leonardozilli/CognitiveBiasOntology/HumorEffect#MentalContent"/>
    </owl:NamedIndividual>
</rdf:RDF>



<!-- Generated by the OWL API (version 4.5.25.2023-02-15T19:15:49Z) https://github.com/owlcs/owlapi -->

