@prefix : <https://github.com/leonardozilli/CognitiveBiasOntology/HumorEffect#> .
@prefix fs: <https://w3id.org/framester/data/framestercore/> .
@prefix cbo: <https://github.com/leonardozilli/CognitiveBiasOntology/HumorEffect#> .
@prefix owl: <http://www.w3.org/2002/07/owl#> .
@prefix rdf: <http://www.w3.org/1999/02/22-rdf-syntax-ns#> .
@prefix xml: <http://www.w3.org/XML/1998/namespace> .
@prefix xsd: <http://www.w3.org/2001/XMLSchema#> .
@prefix rdfs: <http://www.w3.org/2000/01/rdf-schema#> .
@base <https://github.com/leonardozilli/CognitiveBiasOntology/HumorEffect> .

<https://github.com/leonardozilli/CognitiveBiasOntology/HumorEffect> rdf:type owl:Ontology ;
                                                                      owl:imports <https://raw.githubusercontent.com/modellingDH/odp_experience/master/owl/cp_experience.owl.ttl> ;
                                                                      <http://purl.org/dc/terms/created> "2023-07-23" ;
                                                                      <http://purl.org/dc/terms/creator> "Leonardo Zilli" ;
                                                                      <http://purl.org/dc/terms/description> "The Humor effect module of the Cognitive Bias Ontology." ;
                                                                      <http://purl.org/dc/terms/title> "Humor effect ontology" ;
                                                                      rdfs:comment """Scenario:
A company creates a humorous television commercial for their product. The funny storyline and witty dialogue engage viewers, making the advertisement more memorable. As a result, consumers are more likely to remember the product and its key features when making purchasing decisions.""" ,
                                                                                   "The humor effect is the tendencye of humorous material to be better remembered than common material." .

#################################################################
#    Annotation properties
#################################################################

###  http://purl.org/dc/terms/created
<http://purl.org/dc/terms/created> rdf:type owl:AnnotationProperty .


#################################################################
#    Classes
#################################################################

###  https://github.com/leonardozilli/CognitiveBiasOntology/HumorEffect#Humor
cbo:Humor rdf:type owl:Class ;
          rdfs:subClassOf fs:Feeling .


###  https://github.com/leonardozilli/CognitiveBiasOntology/HumorEffect#HumorousContent
cbo:HumorousContent rdf:type owl:Class ;
                    owl:equivalentClass fs:Prominence ;
                    rdfs:subClassOf cbo:MentalContent .


###  https://github.com/leonardozilli/CognitiveBiasOntology/HumorEffect#MentalContent
cbo:MentalContent rdf:type owl:Class ;
                  rdfs:subClassOf <http://modellingdh.github.io/ont/odp/term/Prompt> .


###  https://w3id.org/framester/data/framestercore/ExperiencerObj
fs:ExperiencerObj rdf:type owl:Class ;
                  rdfs:subClassOf <http://modellingdh.github.io/ont/odp/term/Engagement> ;
                  rdfs:comment "Some phenomenon (the Stimulus) provokes a particular emotion in an Experiencer. Nightmare on Elm Street scared me silly." .


###  https://w3id.org/framester/data/framestercore/Feeling
fs:Feeling rdf:type owl:Class ;
           rdfs:subClassOf <http://modellingdh.github.io/ont/odp/term/Observation> ;
           rdfs:comment "In this frame an Experiencer experiences an Emotion or is in an Emotional_state." .


###  https://w3id.org/framester/data/framestercore/Memory
fs:Memory rdf:type owl:Class ;
          rdfs:subClassOf <http://ontology.eil.utoronto.ca/icity/ActivitySpecification/Activity> ;
          rdfs:comment "This frame is concerned with Cognizers remembering and forgetting mental Content." .


###  https://w3id.org/framester/data/framestercore/Prominence
fs:Prominence rdf:type owl:Class ;
              rdfs:subClassOf fs:Memory ;
              rdfs:comment "An Entity stands out perceptually in comparison to other members of its type." .


#################################################################
#    Individuals
#################################################################

###  https://github.com/leonardozilli/CognitiveBiasOntology/HumorEffect#consumer
cbo:consumer rdf:type owl:NamedIndividual ,
                      <http://www.ontologydesignpatterns.org/cp/owl/persons.owl#Person> ;
             <http://modellingdh.github.io/ont/odp/term/isEngagedIn> cbo:emotional_stimulus .


###  https://github.com/leonardozilli/CognitiveBiasOntology/HumorEffect#decoded_prominent_memory
cbo:decoded_prominent_memory rdf:type owl:NamedIndividual ,
                                      fs:Prominence .


###  https://github.com/leonardozilli/CognitiveBiasOntology/HumorEffect#emotional_stimulus
cbo:emotional_stimulus rdf:type owl:NamedIndividual ,
                                fs:ExperiencerObj ;
                       <http://modellingdh.github.io/ont/odp/term/inActivity> cbo:memory_encoding .


###  https://github.com/leonardozilli/CognitiveBiasOntology/HumorEffect#humorous_advertisement
cbo:humorous_advertisement rdf:type owl:NamedIndividual ,
                                    cbo:HumorousContent ;
                           <http://modellingdh.github.io/ont/odp/term/producedObservation> cbo:laugh .


###  https://github.com/leonardozilli/CognitiveBiasOntology/HumorEffect#laugh
cbo:laugh rdf:type owl:NamedIndividual ,
                   cbo:Humor ;
          <http://modellingdh.github.io/ont/odp/term/isReflectionOn> cbo:emotional_stimulus .


###  https://github.com/leonardozilli/CognitiveBiasOntology/HumorEffect#memory_encoding
cbo:memory_encoding rdf:type owl:NamedIndividual ,
                             fs:Memory .


###  https://github.com/leonardozilli/CognitiveBiasOntology/HumorEffect#mundane_advertisement
cbo:mundane_advertisement rdf:type owl:NamedIndividual ,
                                   cbo:MentalContent .


###  Generated by the OWL API (version 4.5.25.2023-02-15T19:15:49Z) https://github.com/owlcs/owlapi
